PurescriptLanguageCstParser/Types/Expr/Rec/LawfulFunctorMapId.lean
@@ -9,11 +9,11 @@ public import PurescriptLanguageCstParser.Types.Expr.Rec.Basic
 public import PurescriptLanguageCstParser.Types.Expr.Rec.Simp
 public import PurescriptLanguageCstParser.Types.Expr.Rec.Functor
 @[expose] public section
-namespace PureScript.CST.Types
+namespace PurescriptLanguageCstParser.Types
 
 open NonEmpty.CorrectByConstruction.Array
 open NonEmpty.String
-open PureScript.CST.Types
+open PurescriptLanguageCstParser.Types
 
 -- ╔══════════════════════════════════════════════════════════════════╗
 -- ║  id_map theorems                                                 ║
@@ -402,4 +402,4 @@ mutual
     all_goals try decreasing_trivial
 end
 
-end PureScript.CST.Types
+end PurescriptLanguageCstParser.Types
